@prefix : <https://www.w3.org/2019/wot/modbus#> .
@prefix om: <http://www.ontology-of-units-of-measure.org/resource/om-2/> .
@prefix dct: <http://purl.org/dc/terms/> .
@prefix owl: <http://www.w3.org/2002/07/owl#> .
@prefix rdf: <http://www.w3.org/1999/02/22-rdf-syntax-ns#> .
@prefix xml: <http://www.w3.org/XML/1998/namespace> .
@prefix xsd: <http://www.w3.org/2001/XMLSchema#> .
@prefix rdfs: <http://www.w3.org/2000/01/rdf-schema#> .
@prefix vann: <http://purl.org/vocab/vann/> .
@prefix schema: <http://schema.org/> .
@prefix binding: <https://www.w3.org/2019/wot/binding#> .
@base <https://www.w3.org/2019/wot/modbus> .

<https://www.w3.org/2019/wot/modbus> rdf:type owl:Ontology ;
                                      dct:author _:genid1 ;
                                      dct:contributor _:genid1 ;
                                      vann:preferredNamespacePrefix "modv" ;
                                      vann:preferredNamespaceUri : ;
                                      rdfs:comment "Vocabulary to represent Modbus messages in RDF."@en ;
                                      rdfs:label "Modbus in RDF"@en .

_:genid1 rdf:type schema:Person ;
          schema:name "Jakob MÃ¼ller" .

#################################################################
#    Annotation properties
#################################################################

###  http://purl.org/dc/terms/author
dct:author rdf:type owl:AnnotationProperty .


###  http://purl.org/dc/terms/contributor
dct:contributor rdf:type owl:AnnotationProperty .


###  http://purl.org/vocab/vann/preferredNamespacePrefix
vann:preferredNamespacePrefix rdf:type owl:AnnotationProperty .


###  http://purl.org/vocab/vann/preferredNamespaceUri
vann:preferredNamespaceUri rdf:type owl:AnnotationProperty .


###  http://schema.org/name
schema:name rdf:type owl:AnnotationProperty .


###  http://www.ontology-of-units-of-measure.org/resource/om-2/usesUnit
om:usesUnit rdf:type owl:AnnotationProperty .


###  https://www.w3.org/2019/wot/binding#assignment
binding:assignment rdf:type owl:AnnotationProperty .


###  https://www.w3.org/2019/wot/modbus#writeValue
:writeValue rdf:type owl:AnnotationProperty ;
            rdfs:range xsd:integer ;
            rdfs:domain :RequestOption .


#################################################################
#    Datatypes
#################################################################

###  https://www.w3.org/2019/wot/modbus#RequestOption
:RequestOption rdf:type rdfs:Datatype .


#################################################################
#    Object Properties
#################################################################

###  https://www.w3.org/2019/wot/modbus#encodingOption
:encodingOption rdf:type owl:ObjectProperty ;
                rdfs:domain :Request .


###  https://www.w3.org/2019/wot/modbus#entity
:entity rdf:type owl:ObjectProperty ;
        rdfs:domain :Request ;
        rdfs:range :Entity ;
        rdfs:comment "A registry type to let the runtime automatically detect the right function code"@en ;
        rdfs:isDefinedBy <https://www.w3.org/2019/wot/modbus> ;
        rdfs:label "Entity"@en .


###  https://www.w3.org/2019/wot/modbus#firstDWordLow
:firstDWordLow rdf:type owl:ObjectProperty ;
               rdfs:domain :Request .


###  https://www.w3.org/2019/wot/modbus#firstWordLow
:firstWordLow rdf:type owl:ObjectProperty ;
              rdfs:domain :Request .


###  https://www.w3.org/2019/wot/modbus#function
:function rdf:type owl:ObjectProperty ;
          rdfs:domain :Request ;
          rdfs:range :FunctionCode ,
                     :FunctionName ;
          rdfs:comment "Function Code sent by the master in every request. Specifying the desired interaction."@en ;
          rdfs:isDefinedBy <https://www.w3.org/2019/wot/modbus> ;
          rdfs:label "Function"@en .


###  https://www.w3.org/2019/wot/modbus#functionCode
:functionCode rdf:type owl:ObjectProperty ;
              rdfs:domain :FunctionName ;
              rdfs:range :FunctionCode ;
              rdfs:label "Function code of a function Name"@en .


###  https://www.w3.org/2019/wot/modbus#functionName
:functionName rdf:type owl:ObjectProperty ;
              rdfs:domain :FunctionCode ;
              rdfs:range :FunctionName ;
              rdfs:label "Function name of a function Code"@en .


###  https://www.w3.org/2019/wot/modbus#length
:length rdf:type owl:ObjectProperty ;
        rdfs:domain :Request .


###  https://www.w3.org/2019/wot/modbus#offset
:offset rdf:type owl:ObjectProperty ;
        rdfs:domain :Request .


###  https://www.w3.org/2019/wot/modbus#options
:options rdf:type owl:ObjectProperty ;
         rdfs:domain :Request .


###  https://www.w3.org/2019/wot/modbus#pollingTime
:pollingTime rdf:type owl:ObjectProperty ;
             rdfs:domain :Request .


###  https://www.w3.org/2019/wot/modbus#responseCode
:responseCode rdf:type owl:ObjectProperty ;
              rdfs:domain :Response ;
              rdfs:range :ResponseCode ;
              rdfs:comment "Response Code returned by the slave after a request"@en ;
              rdfs:isDefinedBy <https://www.w3.org/2019/wot/modbus> ;
              rdfs:label "Response Code"@en .


###  https://www.w3.org/2019/wot/modbus#timeout
:timeout rdf:type owl:ObjectProperty ;
         rdfs:domain :Request .


###  https://www.w3.org/2019/wot/modbus#unitID
:unitID rdf:type owl:ObjectProperty ;
        rdfs:domain :Request .


###  https://www.w3.org/2019/wot/modbus#writeValue
:writeValue rdf:type owl:ObjectProperty .


###  https://www.w3.org/2019/wot/modbus#zeroBasedAddressing
:zeroBasedAddressing rdf:type owl:ObjectProperty ;
                     rdfs:domain :Request .


#################################################################
#    Data properties
#################################################################

###  https://www.w3.org/2019/wot/modbus#firstDWordLow
:firstDWordLow rdf:type owl:DatatypeProperty ;
               rdfs:range xsd:boolean .


###  https://www.w3.org/2019/wot/modbus#firstWordLow
:firstWordLow rdf:type owl:DatatypeProperty ;
              rdfs:range xsd:boolean .


###  https://www.w3.org/2019/wot/modbus#length
:length rdf:type owl:DatatypeProperty ;
        rdfs:range xsd:integer .


###  https://www.w3.org/2019/wot/modbus#offset
:offset rdf:type owl:DatatypeProperty ;
        rdfs:range xsd:integer .


###  https://www.w3.org/2019/wot/modbus#options
:options rdf:type owl:DatatypeProperty ;
         rdfs:range :RequestOption .


###  https://www.w3.org/2019/wot/modbus#pollingTime
:pollingTime rdf:type owl:DatatypeProperty ;
             rdfs:range xsd:integer .


###  https://www.w3.org/2019/wot/modbus#timeout
:timeout rdf:type owl:DatatypeProperty ;
         rdfs:range xsd:integer .


###  https://www.w3.org/2019/wot/modbus#unitID
:unitID rdf:type owl:DatatypeProperty ;
        rdfs:range xsd:integer .


###  https://www.w3.org/2019/wot/modbus#writeValue
:writeValue rdf:type owl:DatatypeProperty .


###  https://www.w3.org/2019/wot/modbus#zeroBasedAddressing
:zeroBasedAddressing rdf:type owl:DatatypeProperty ;
                     rdfs:range xsd:boolean .


#################################################################
#    Classes
#################################################################

###  http://schema.org/Person
schema:Person rdf:type owl:Class .


###  http://www.w3.org/2001/XMLSchema#string
xsd:string rdf:type owl:Class .


###  https://www.w3.org/2019/wot/modbus#Code
:Code rdf:type owl:Class ;
      rdfs:comment "In a Modbus Message the content of a requested operation (sent by client to server) or of a response (elaborated by the server and sent to client) is expressed with a specific code, that could be a normal one ( function code) or an exception one (exception code)."@en ;
      rdfs:label "Code" .


###  https://www.w3.org/2019/wot/modbus#Entity
:Entity rdf:type owl:Class ;
        owl:equivalentClass [ rdf:type owl:Class ;
                              owl:oneOf ( :Coil
                                          :DiscreteInput
                                          :HoldingRegister
                                          :InputRegister
                                        )
                            ] ;
        rdfs:comment "A Modbus registry type"@en ;
        rdfs:label "Entity"@en .


###  https://www.w3.org/2019/wot/modbus#FunctionCode
:FunctionCode rdf:type owl:Class ;
              owl:equivalentClass [ rdf:type owl:Class ;
                                    owl:oneOf ( <https://www.w3.org/2019/wot/modbus/functionCode#1>
                                                <https://www.w3.org/2019/wot/modbus/functionCode#15>
                                                <https://www.w3.org/2019/wot/modbus/functionCode#16>
                                                <https://www.w3.org/2019/wot/modbus/functionCode#2>
                                                <https://www.w3.org/2019/wot/modbus/functionCode#3>
                                                <https://www.w3.org/2019/wot/modbus/functionCode#4>
                                                <https://www.w3.org/2019/wot/modbus/functionCode#43>
                                                <https://www.w3.org/2019/wot/modbus/functionCode#5>
                                                <https://www.w3.org/2019/wot/modbus/functionCode#6>
                                              )
                                  ] ;
              rdfs:subClassOf :Code ;
              rdfs:comment "Function Code class represents the value of the function field in a Modbus frame. Each operation identified with a code also have a corresponding human readable name."@en ;
              rdfs:label "Function Code"@en .


###  https://www.w3.org/2019/wot/modbus#FunctionName
:FunctionName rdf:type owl:Class ;
              owl:equivalentClass [ rdf:type owl:Class ;
                                    owl:oneOf ( :readCoil
                                                :readDiscreteInput
                                                :readHoldingRegisters
                                                :readInputRegisters
                                                :writeMultipleCoils
                                                :writeMultipleHoldingRegisters
                                                :writeSingleCoil
                                                :writeSingleHoldingRegister
                                              )
                                  ] ;
              rdfs:comment "A Modbus human readable function name"@en ;
              rdfs:label "Function Name"@en .


###  https://www.w3.org/2019/wot/modbus#Message
:Message rdf:type owl:Class ;
         rdfs:comment "A Modbus Message class represents the comunication between client and server"@en ;
         rdfs:isDefinedBy <https://www.w3.org/2019/wot/modbus> ;
         rdfs:label "A Modbus Message"@en .


###  https://www.w3.org/2019/wot/modbus#Request
:Request rdf:type owl:Class ;
         rdfs:subClassOf :Message ;
         rdfs:comment "A Request message is sent by a client device to a server device. The comunication client/server stats only with a request sent by the client."@en ;
         rdfs:label "Request"@en .


###  https://www.w3.org/2019/wot/modbus#Response
:Response rdf:type owl:Class ;
          rdfs:subClassOf :Message ;
          rdfs:comment "A Response message is sent by a server device to client device in return to a client's query."@en ;
          rdfs:label "Response"@en .


###  https://www.w3.org/2019/wot/modbus#ResponseCode
:ResponseCode rdf:type owl:Class ;
              owl:equivalentClass [ rdf:type owl:Class ;
                                    owl:oneOf ( <https://www.w3.org/2019/wot/modbus/errorCode#01>
                                                <https://www.w3.org/2019/wot/modbus/errorCode#02>
                                                <https://www.w3.org/2019/wot/modbus/errorCode#03>
                                                <https://www.w3.org/2019/wot/modbus/errorCode#04>
                                                <https://www.w3.org/2019/wot/modbus/errorCode#05>
                                                <https://www.w3.org/2019/wot/modbus/errorCode#06>
                                              )
                                  ] ;
              rdfs:subClassOf :Code ;
              rdfs:comment "In case of Exception Response, the server returns an Exception Code in the data field. Exception Code defines the server condition that caused the exception. Each status identified with a code also have a corresponding human readable name."@en ;
              rdfs:label "Exception Code"@en .


#################################################################
#    Individuals
#################################################################

###  https://www.w3.org/2019/wot/modbus#Coil
:Coil rdf:type owl:NamedIndividual ,
               :Entity ;
      rdfs:comment "Represent a modbus coil register.  These entities can be read or written"@en ;
      rdfs:label "Coil"@en .


###  https://www.w3.org/2019/wot/modbus#DiscreteInput
:DiscreteInput rdf:type owl:NamedIndividual ,
                        :Entity ;
               rdfs:comment "Represent a modbus discrete input. These entities can only be read"@en ;
               rdfs:label "Discrete Input"@en .


###  https://www.w3.org/2019/wot/modbus#HoldingRegister
:HoldingRegister rdf:type owl:NamedIndividual ,
                          :Entity ;
                 rdfs:comment "Represent a modbus holding register.  These entities can be read or written"@en ;
                 rdfs:label "Holding Register"@en .


###  https://www.w3.org/2019/wot/modbus#InputRegister
:InputRegister rdf:type owl:NamedIndividual ,
                        :Entity ;
               rdfs:comment "Represent a modbus input register. These entities can only be read"@en ;
               rdfs:label "Input Register"@en .


###  https://www.w3.org/2019/wot/modbus#encodingOption
:encodingOption rdf:type owl:NamedIndividual ,
                         xsd:string .


###  https://www.w3.org/2019/wot/modbus#readCoil
:readCoil rdf:type owl:NamedIndividual ,
                   :FunctionName ;
          :functionCode <https://www.w3.org/2019/wot/modbus/functionCode#1> ;
          rdfs:comment "Read a single coil (i.e. boolean/bit access) value. Usually in the address range 00001-09999"@en ;
          rdfs:label "Read Single Coils"@en .


###  https://www.w3.org/2019/wot/modbus#readDiscreteInput
:readDiscreteInput rdf:type owl:NamedIndividual ,
                            :FunctionName ;
                   :functionCode <https://www.w3.org/2019/wot/modbus/functionCode#2> ;
                   rdfs:comment "Read Physical Discrete Inputs (bit access). Address range 10001-19999"@en ;
                   rdfs:label "Read Discrete Inputs"@en .


###  https://www.w3.org/2019/wot/modbus#readHoldingRegisters
:readHoldingRegisters rdf:type owl:NamedIndividual ,
                               :FunctionName ;
                      :functionCode <https://www.w3.org/2019/wot/modbus/functionCode#3> ;
                      rdfs:comment "Read Multiple Holding Registers (16 bit access). Address range 40001-49999"@en ;
                      rdfs:label "Read Multiple Holding Registers"@en .


###  https://www.w3.org/2019/wot/modbus#readInputRegisters
:readInputRegisters rdf:type owl:NamedIndividual ,
                             :FunctionName ;
                    :functionCode <https://www.w3.org/2019/wot/modbus/functionCode#4> ;
                    rdfs:comment "Read Multiple Physical Input Registers (16 bits). Address range 30001-39999"@en ;
                    rdfs:label "Read Multiple Input Registers"@en .


###  https://www.w3.org/2019/wot/modbus#writeMultipleCoils
:writeMultipleCoils rdf:type owl:NamedIndividual ,
                             :FunctionName ;
                    :functionCode <https://www.w3.org/2019/wot/modbus/functionCode#15> ;
                    rdfs:comment "Write Multiple Physical Coils (internal bits). Address range 00001-09999"@en ;
                    rdfs:label "Write Multiple Coils"@en .


###  https://www.w3.org/2019/wot/modbus#writeMultipleHoldingRegisters
:writeMultipleHoldingRegisters rdf:type owl:NamedIndividual ,
                                        :FunctionName ;
                               :functionCode <https://www.w3.org/2019/wot/modbus/functionCode#16> ;
                               rdfs:comment "Write Multiple Holding Registers (output registers, 16 bit). Address range 40001-49999"@en ;
                               rdfs:label "Write Multiple Holding Registers"@en .


###  https://www.w3.org/2019/wot/modbus#writeSingleCoil
:writeSingleCoil rdf:type owl:NamedIndividual ,
                          :FunctionName ;
                 :functionCode <https://www.w3.org/2019/wot/modbus/functionCode#5> ;
                 rdfs:comment "Write Single Physical Coil (internal bit). Address range 00001-09999"@en ;
                 rdfs:label "Write Single Coil"@en .


###  https://www.w3.org/2019/wot/modbus#writeSingleHoldingRegister
:writeSingleHoldingRegister rdf:type owl:NamedIndividual ,
                                     :FunctionName ;
                            :functionCode <https://www.w3.org/2019/wot/modbus/functionCode#6> ;
                            rdfs:comment "Write Single HoldingRegister (internal bits). Address range 40001-49999"@en ;
                            rdfs:label "Write Single HoldingRegister"@en .


###  https://www.w3.org/2019/wot/modbus/errorCode#01
<https://www.w3.org/2019/wot/modbus/errorCode#01> rdf:type owl:NamedIndividual ,
                                                           :ResponseCode ;
                                                  rdfs:comment "Function code received in the query is not recognized or allowed by slave"@en ;
                                                  rdfs:label "ILLEGAL FUNCTION"@en .


###  https://www.w3.org/2019/wot/modbus/errorCode#02
<https://www.w3.org/2019/wot/modbus/errorCode#02> rdf:type owl:NamedIndividual ,
                                                           :ResponseCode ;
                                                  rdfs:comment "Data address of some or all the required entities are not allowed or do not exist in slave"@en ;
                                                  rdfs:label "ILLEGAL DATA ADDRESS"@en .


###  https://www.w3.org/2019/wot/modbus/errorCode#03
<https://www.w3.org/2019/wot/modbus/errorCode#03> rdf:type owl:NamedIndividual ,
                                                           :ResponseCode ;
                                                  rdfs:comment "Value is not accepted by slave"@en ;
                                                  rdfs:label "ILLEGAL DATA VALUE"@en .


###  https://www.w3.org/2019/wot/modbus/errorCode#04
<https://www.w3.org/2019/wot/modbus/errorCode#04> rdf:type owl:NamedIndividual ,
                                                           :ResponseCode ;
                                                  rdfs:comment "An unrecoverable error occurred while the slave was attempting to perform the requested action"@en ;
                                                  rdfs:label "SLAVEDEVICE FAILURE" .


###  https://www.w3.org/2019/wot/modbus/errorCode#05
<https://www.w3.org/2019/wot/modbus/errorCode#05> rdf:type owl:NamedIndividual ,
                                                           :ResponseCode ;
                                                  rdfs:comment "The server has accepted the request and is processing it, but a long duration of time will be required to do so. This response is returned to prevent a timeout error from occurring in the client. The client can next issue a Poll Program Complete  message to determine if processing is completed"@en ;
                                                  rdfs:label "ACKNOWLEDGE" .


###  https://www.w3.org/2019/wot/modbus/errorCode#06
<https://www.w3.org/2019/wot/modbus/errorCode#06> rdf:type owl:NamedIndividual ,
                                                           :ResponseCode ;
                                                  rdfs:comment "Slave is engaged in processing a long-duration command. Master should retry later "@en ;
                                                  rdfs:label "SLAVEDEVICE BUISY"@en .


###  https://www.w3.org/2019/wot/modbus/functionCode#1
<https://www.w3.org/2019/wot/modbus/functionCode#1> rdf:type owl:NamedIndividual ,
                                                             :FunctionCode ;
                                                    :functionName :readCoil ;
                                                    rdfs:comment "Read a single coil (i.e. boolean/bit access) value. Usually in the address range 00001-09999"@en ;
                                                    rdfs:label "Read Single Coils"@en .


###  https://www.w3.org/2019/wot/modbus/functionCode#15
<https://www.w3.org/2019/wot/modbus/functionCode#15> rdf:type owl:NamedIndividual ,
                                                              :FunctionCode ;
                                                     :functionName :writeMultipleCoils ;
                                                     rdfs:comment "Write Multiple Physical Coils (internal bits). Address range 00001-09999"@en ;
                                                     rdfs:label "Write Multiple Coils"@en .


###  https://www.w3.org/2019/wot/modbus/functionCode#16
<https://www.w3.org/2019/wot/modbus/functionCode#16> rdf:type owl:NamedIndividual ,
                                                              :FunctionCode ;
                                                     :functionName :writeMultipleHoldingRegisters ;
                                                     rdfs:comment "Write Multiple Holding Registers (output registers, 16 bit). Address range 40001-49999"@en ;
                                                     rdfs:label "Write Multiple Holding Registers"@en .


###  https://www.w3.org/2019/wot/modbus/functionCode#2
<https://www.w3.org/2019/wot/modbus/functionCode#2> rdf:type owl:NamedIndividual ,
                                                             :FunctionCode ;
                                                    :functionName :readDiscreteInput ;
                                                    rdfs:comment "Read Physical Discrete Inputs (bit access). Address range 10001-19999"@en ;
                                                    rdfs:label "Read Discrete Inputs"@en .


###  https://www.w3.org/2019/wot/modbus/functionCode#3
<https://www.w3.org/2019/wot/modbus/functionCode#3> rdf:type owl:NamedIndividual ,
                                                             :FunctionCode ;
                                                    :functionName :readHoldingRegisters ;
                                                    rdfs:comment "Read Multiple Holding Registers (16 bit access). Address range 40001-49999"@en ;
                                                    rdfs:label "Read Multiple Holding Registers"@en .


###  https://www.w3.org/2019/wot/modbus/functionCode#4
<https://www.w3.org/2019/wot/modbus/functionCode#4> rdf:type owl:NamedIndividual ,
                                                             :FunctionCode ;
                                                    :functionName :readInputRegisters ;
                                                    rdfs:comment "Read Multiple Physica Input Registers (16 bits). Address range 30001-39999"@en ;
                                                    rdfs:label "Read Multiple Input Registers"@en .


###  https://www.w3.org/2019/wot/modbus/functionCode#43
<https://www.w3.org/2019/wot/modbus/functionCode#43> rdf:type owl:NamedIndividual ,
                                                              :FunctionCode ;
                                                     rdfs:comment "Read Device Identification for diagnostic purposes. Avaiable in the majority of Modbus implementations"@en ;
                                                     rdfs:label "Read Device Identification"@en .


###  https://www.w3.org/2019/wot/modbus/functionCode#5
<https://www.w3.org/2019/wot/modbus/functionCode#5> rdf:type owl:NamedIndividual ,
                                                             :FunctionCode ;
                                                    :functionName :writeSingleCoil ;
                                                    rdfs:comment "Write Single Physical Coil (internal bit). Address range 00001-09999"@en ;
                                                    rdfs:label "Write Single Coil"@en .


###  https://www.w3.org/2019/wot/modbus/functionCode#6
<https://www.w3.org/2019/wot/modbus/functionCode#6> rdf:type owl:NamedIndividual ,
                                                             :FunctionCode ;
                                                    :functionName :writeSingleHoldingRegister ;
                                                    rdfs:comment "Write Single HoldingRegister (internal bits). Address range 40001-49999"@en ;
                                                    rdfs:label "Write Single HoldingRegister"@en .


_:genid1 rdf:type schema:Person ;
         schema:name "Jakob MÃ¼ller" .

#################################################################
#    Annotations
#################################################################

:encodingOption rdfs:label "Byte Encoding"@en ;
                 rdfs:comment "Little Endian or Big Endian encoding of bytes, i.e. the bit order within each register. Default is Big Endian"@en .


:firstDWordLow rdfs:comment "Data encoding for 64-bit values; same as firstWordLow but based on DWORDS (i.e. 2 registers) instead of WORDS (1 register)"@en ;
               rdfs:label "First DoubleWord Low Flag"@en .


:firstWordLow rdfs:label "First Word Low Flag"@en ;
              rdfs:comment "Data encoding for 32-bit values to chose which of the register is the low value"@en .


:length rdfs:label "Length of requested registers/coils"@en ;
        rdfs:comment "Specifies the amount of either registers or coils to be read/written"@en .


:offset rdfs:label "Offset"@en ;
        rdfs:comment "Specifies the starting address of the modbus operations"@en ;
        binding:assignment binding:required .


:options rdfs:comment "Request Options"@en ;
         rdfs:label "Request Options"@en .


:pollingTime rdfs:label "Modbus TCP maximum polling rate"@en ;
             rdfs:comment "The Modbus specification does not define a maximum or minimum allowed polling rate, however specific implementations might introduce such limits. Defined as integer of milliseconds." ;
             om:usesUnit om:milliseconds .


:timeout rdfs:label "Modbus response maximum waiting time"@en ;
         rdfs:comment "Defines how much time the runtime should wait until it receives a reply from the device." ;
         om:usesUnit om:milliseconds .


:unitID rdfs:label "UnitID"@en ;
        rdfs:comment "The Unit ID is usually not needed for ModbusTCP, since the IP-address works as unique identifier, but for compability reasons still often included" .


:writeValue rdfs:comment "The value to write to the register or coil, encoded as integer, omitted and ignored for reading operations"@en ;
            rdfs:label "Write Value"@en .


:zeroBasedAddressing rdfs:label "Zero Based Addressing Flag"@en ;
                     rdfs:comment "Modbus implementations can differ in the way addressing works, as the first coil/register can be either referred to as '0' or '1'. Default is '0'."@en .


###  Generated by the OWL API (version 4.5.9.2019-02-01T07:24:44Z) https://github.com/owlcs/owlapi
